theories/Generic.v
@@ -1,4 +1,4 @@
-Require Import List.
+Require Import Coq.Lists.List.
 Require Import ExtLib.Data.Vector.
 Require Import ExtLib.Data.HList.
 
